\section{Parallel algorithms for separable sums}
\label{sec:sepsum}
\begin{figure}[H]
  \footnotesize
  \centering
  \begin{multicols}{2}
    \begin{minipage}{0.49\textwidth}
      \begin{algorithm}[H]
        \DontPrintSemicolon
        \caption{\hogwild{} for separable sums}
        \label{alg:hogwildsepsum}
        \lFor{$e\in V$}{$\hat{A}(e) = 0$}\;
        \lFor{$l = 1,\dots,L$}{$\hat\alpha_l = 0$, $\hat\beta_l = \sum_{e\in S_l}w_l(e)$}\;
        \ParForAll{$p \in \set{1, \ldots, P}$}{
          \While{$\exists$ element to process}{
            $e = $ next element to process\;
            $\Delta_+^{\max}(e) = -\lambda v(e) + \sum_{S_l\ni e} g(\hat\alpha_l + w_l(e)) - g(\hat\alpha_l)$\;
            $\Delta_-^{\max}(e) = +\lambda v(e) + \sum_{S_l\ni e} g(\hat\beta_l   - w_l(e)) - g(\hat\beta_l)$\;
            Draw $u_e\sim Unif(0,1)$\;
            \If {$u_e<\frac{[\Delta_{+}^{\max}(e)]_+}{[\Delta_{+}^{\min}(e)]_+ + [\Delta_{-}^{\max}(e)]_+}$}{
              $\hat{A}(e) \leftarrow 1$\;
              \lFor{$l: e \in S_l$}{
                $\hat\alpha_l \leftarrow \hat\alpha_l + w_l(e)$
              }
            }\lElse{
              \lFor{$l: e \in S_l$}{
                $\hat\beta_l \leftarrow \hat\beta_l - w_l(e)$
              }
            }
          }
        }
      \end{algorithm}
      \begin{algorithm}[H]
        \DontPrintSemicolon
        \caption{\occ{} validate for separable sums}
        \label{alg:occsepsumvalidate}
        \WaitUntil $\forall j < i$, processed$(j) = true$\;
        $\Delta_+^{\text{exact}}(e) = -\lambda v(e) + \sum_{S_l\ni e} g(\hat\alpha_l + w_l(e)) - g(\hat\alpha_l)$\;
        $\Delta_-^{\text{exact}}(e) = +\lambda v(e) + \sum_{S_l\ni e} g(\hat\beta_l   - w_l(e)) - g(\hat\beta_l)$\;
        \lIf {$u_e < \frac{[\Delta_+^{\text{exact}}(e)]_+}{[\Delta_+^{\text{exact}}(e)]_+ + [\Delta_-^{\text{exact}}(e)]_+}$}{
          result$(i) \leftarrow 1$\;
        }\lElse{
          result$(i) \leftarrow -1$\;
        }
      \end{algorithm}

    \end{minipage}

    \begin{minipage}{0.49\textwidth}
      \begin{algorithm}[H]
        \DontPrintSemicolon
        \caption{\occ{} for separable sums}
        \label{alg:occsepsum}
        \lFor{$e\in V$}{$\hat{A}(e) = \tilde{A}(e) = 0$, $\hat{B}(e) = \tilde{B}(e) = 1$}\;
        \For{$l = 1,\dots,L$}{
          $\hat\alpha_l = \tilde\alpha_l = 0$\;
          $\hat\beta_l = \tilde\beta_l = \sum_{e\in S_l}w_l(e)$\;
        }
        \lFor{$i = 1,\dots,|V|$}{result$(i) = 0$}\;
        \lFor{$i = 1,\dots,|V|$}{processed$(i) = false$}\;
        $\iota = 0$\;
        \ParForAll{$p \in \set{1, \ldots, P}$}{
          \While{$\exists$ element to process}{
            $e = $ next element to process\;
            $\tilde{A}(e) \leftarrow 1$\;
            $\tilde{B}(e) \leftarrow 0$\;
            \For{$l: e \in S_l$}{
              $\tilde\alpha_l \leftarrow \tilde\alpha_l + w_l(e)$\;
              $\tilde\beta_l  \leftarrow \tilde\beta_l  - w_l(e)$\;
            }
            $i = \iota$; $\iota \leftarrow \iota + 1$\;
            $\Delta_+^{\min}(e) = -\lambda v(e) + \sum_{S_l\ni e} g(\tilde\alpha_l) - g(\tilde\alpha_l - w_l(e))$\;
            $\Delta_+^{\max}(e) = -\lambda v(e) + \sum_{S_l\ni e} g(\hat\alpha_l + w_l(e)) - g(\hat\alpha_l)$\;
            $\Delta_-^{\min}(e) = +\lambda v(e) + \sum_{S_l\ni e} g(\tilde\beta_l) - g(\tilde\beta_l + w_l(e))$\;
            $\Delta_-^{\max}(e) = +\lambda v(e) + \sum_{S_l\ni e} g(\hat\beta_l   - w_l(e)) - g(\hat\beta_l)$\;
            Draw $u_e \sim Unif(0,1)$\;
            \If {$u_e < \frac{[\Delta_+^{\min}(e)]_+}{[\Delta_+^{\min}(e)]_+ + [\Delta_-^{\max}(e)]_+}$}{
              result$(i) \leftarrow 1$\;
            }\ElseIf {$u_e > \frac{[\Delta_+^{\max}(e)]_+}{[\Delta_+^{\max}(e)]_+ + [\Delta_-^{\min}(e)]_+}$}{
              result$(i) \leftarrow -1$\;
            }
            \WaitUntil $\forall j<i$, result$(j) \neq 0$\;
            \lIf {result$(i) = 0$}{validate($p$, $e$, $i$)}\;
            \If {result$(i) = 1$}{
              $\hat{A}(e)   \leftarrow 1$\;
              $\tilde{B}(e) \leftarrow 1$\;
              \For{$l: e \in S_l$}{
                $\hat\alpha_l   \leftarrow \hat\alpha_l   + w_l(e)$\;
                $\tilde\beta_l  \leftarrow \tilde\beta_l  + w_l(e)$\;
              }
            }\Else{
              $\tilde{A}(e) \leftarrow 0$\;
              $\hat{B}(e)   \leftarrow 0$\;
              \For{$l: e \in S_l$}{
                $\tilde\alpha_l \leftarrow \tilde\alpha_l - w_l(e)$\;
                $\hat\beta_l    \leftarrow \hat\beta_l    - w_l(e)$\;
              }
            }
            processed$(i) = true$\;
          }
        }
      \end{algorithm}
    \end{minipage}
  \end{multicols}
\end{figure}

For some functions $F$, we can maintain sketches / statistics to aid the computation of $\Delta_+^{\max}$, $\Delta_-^{\max}$, $\Delta_+^{\min}$, $\Delta_-^{\min}$.
In particular, we consider functions of the form
$F(X) = \sum_{l=1}^L g\left(\sum_{i\in X\cup S_l} w_l(i)\right) - \lambda\sum_{i\in X} v(i)$,
where $S_l \subseteq V$ are (possibly overlapping) groups of elements in the ground set, $g$ is a non-decreasing concave scalar function, and $w_l(i)$ and $v(i)$ are non-negative scalar weights.
It is easy to see that
$
F(X \cup e) - F(X) = \sum_{l: e\in S_l} \left[g\left(w_l(e) + \sum_{i\in X\cup S_l} w_l(i)\right) - g\left(\sum_{i\in X\cup S_l} w_l(i)\right)\right] - \lambda v(e)$.
Define
%  $\hat\alpha_l              = \sum_{j\in \hat{A}\cup S_l} w_l(j)$,
% $\hat\alpha_{l,e}          = \sum_{j\in \hat{A}_e\cup S_l} w_l(j)$,
% $\alpha_l^{\iota(e)-1} = \sum_{j\in A^{\iota(e)-1}\cup S_l} w_l(j)$.
%
%  $\hat\beta_l              = \sum_{j\in \hat{B}\cup S_l} w_l(j)$,
% $\hat\beta_{l,e}          = \sum_{j\in \hat{B}_e\cup S_l} w_l(j)$,
% $\beta_l^{\iota(e)-1} = \sum_{j\in B^{\iota(e)-1}\cup S_l} w_l(j)$.
%
\begin{align*}
  \hat\alpha_l              &= \sum_{j\in \hat{A}\cup S_l} w_l(j),
& \hat\alpha_{l,e}          &= \sum_{j\in \hat{A}_e\cup S_l} w_l(j),
& \alpha_l^{\iota(e)-1} &= \sum_{j\in A^{\iota(e)-1}\cup S_l} w_l(j).\\
  \hat\beta_l              &= \sum_{j\in \hat{B}\cup S_l} w_l(j),
& \hat\beta_{l,e}          &= \sum_{j\in \hat{B}_e\cup S_l} w_l(j),
& \beta_l^{\iota(e)-1} &= \sum_{j\in B^{\iota(e)-1}\cup S_l} w_l(j).
\end{align*}


\subsection{\hogwild{} for separable sums $F$}
Algorithm \ref{alg:hogwildsepsum} updates $\hat\alpha_l$ and $\hat\beta_l$, and computes $\Delta_+^{\max}(e)$ and $\Delta_-^{\max}(e)$ using $\hat\alpha_{l,e}$ and $\hat\beta_{l,e}$.
Following arguments analogous to that of Lemma \ref{lem:hog:set_bound}, we can show:

\begin{lem} For each $l$ and $e\in V$, $\hat\alpha_{l,e} \leq \alpha_l^{\iota(e)-1}$ and $\hat\beta_{l,e} \geq \beta_l^{\iota(e)-1}$.
\end{lem}

\begin{cor} Concavity of $g$ implies that $\Delta$'s computed by Algorithm \ref{alg:hogwildsepsum} satisfy
\begin{align*}
\Delta_+^{\max}(e)
&&\geq&& \sum_{S_l\ni e} \left[g(\alpha_l^{\iota(e)-1} + w_l(e)) - g(\alpha_l^{\iota(e)-1})\right] - \lambda v(e)
&&=&& \Delta_+(e),\\
\Delta_-^{\max}(e)
&&\geq&& \sum_{S_l\ni e} \left[g(\beta_l^{\iota(e)-1} - w_l(e)) - g(\beta_l^{\iota(e)-1})\right] + \lambda v(e)
&&=&& \Delta_-(e),
\end{align*}
\end{cor}

\subsection{\occ{} for separable sums $F$}
Analogous to the \hogwild{} algorithm, we maintain $\hat\alpha_l$, $\hat\beta_l$ and additionally $\tilde\alpha_l = \sum_{j\in \tilde{A}\cup S_l} w_l(j)$ and $\tilde\beta_l = \sum_{j \in \tilde{B}\cup S_l} w_l(j)$.
Following the arguments of Lemma \ref{lem:occ:set_bound} and Corollary \ref{cor:occ:delta_bound}, we can show the following.
\begin{lem} $\hat\alpha_{l,e} \leq \alpha^{\iota(e)-1} \leq \tilde\alpha_{l,e} - w_l(e)$ and $\hat\beta_{l,e} \geq \beta^{\iota(e)-1} \geq \tilde\beta_{l,e} + w_l(e)$
\end{lem}

\begin{cor} Concavity of $g$ implies that the $\Delta$'s computed by Algorithm \ref{alg:occsepsum} satisfy:
\begin{align*}
\Delta_+^{\max}(e)
&= - \lambda v(e) + \sum_{S_l \ni e} \left[g(\hat\alpha_{l,e} + w_l(e)) - g(\hat\alpha_{l,e})\right]\\
&\geq - \lambda v(e) + \sum_{S_l \ni e} \left[g(\hat\alpha_l^{\iota(e)-1} + w_l(e)) - g(\hat\alpha_l^{\iota(e)-1})\right]
&&= \Delta_+(e)\\
&\geq - \lambda v(e) + \sum_{S_l \ni e} \left[g(\tilde\alpha_{l,e}) - g(\tilde\alpha_{l,e} - w_l(e))\right]
&&= \Delta_+^{\min}(e),\\
\Delta_-^{\max}(e)
&= \lambda v(e) + \sum_{S_l \ni e} \left[g(\hat\beta_{l,e} - w_l(e)) - g(\hat\beta_{l,e})\right]\\
&\geq \lambda v(e) + \sum_{S_l \ni e} \left[g(\hat\beta_l^{\iota(e)-1} - w_l(e)) - g(\hat\beta_l^{\iota(e)-1})\right]
&&= \Delta_-(e)\\
&\geq \lambda v(e) + \sum_{S_l \ni e} \left[g(\tilde\beta_l^{\iota(e)-1}) - g(\tilde\beta_l^{\iota(e)-1} + w_l(e))\right]
&&= \Delta_-^{\min}(e).
\end{align*}
\end{cor}